Semantic equivalence includes join points!!

CBPV/Equivalence.lean
@@ -205,19 +205,19 @@ theorem ℰ.bwds {m m' n n' B} (rm : m ⇒⋆ m') (rn : n ⇒⋆ n') (h : (m', n
   let ⟨m'', n'', nm', nn', h⟩ := h
   exact ⟨m'', n'', nm'.bwds rm, nn'.bwds rn, h⟩
 
-theorem ℰ.bwdsRejoin {m m' n n' js B} (rm : m ⇒⋆ m') (rn : n ⇒⋆ n') (h : (m', n') ∈ ⟦B⟧ᵉ) : (rejoin m js, rejoin n js) ∈ ⟦B⟧ᵉ := by
+theorem ℰ.bwdsRejoin {m m' n n' js₁ js₂ B} (rm : m ⇒⋆ m') (rn : n ⇒⋆ n') (h : (m', n') ∈ ⟦B⟧ᵉ) : (rejoin m js₁, rejoin n js₂) ∈ ⟦B⟧ᵉ := by
   unfold ℰ at *
   let ⟨m'', n'', nm', nn', h⟩ := h
   refine ⟨m'', n'', nm'.bwdsRejoin rm, nn'.bwdsRejoin rn, h⟩
 
 theorem ℰ.bwd {m m' n n' B} (rm : m ⇒ m') (rn : n ⇒ n') : (m', n') ∈ ⟦B⟧ᵉ → (m, n) ∈ ⟦B⟧ᵉ := ℰ.bwds (.once rm) (.once rn)
-theorem ℰ.bwdRejoin {m m' n n' js B} (rm : m ⇒ m') (rn : n ⇒ n') : (m', n') ∈ ⟦B⟧ᵉ → (rejoin m js, rejoin n js) ∈ ⟦B⟧ᵉ := ℰ.bwdsRejoin (.once rm) (.once rn)
+theorem ℰ.bwdRejoin {m m' n n' js₁ js₂ B} (rm : m ⇒ m') (rn : n ⇒ n') : (m', n') ∈ ⟦B⟧ᵉ → (rejoin m js₁, rejoin n js₂) ∈ ⟦B⟧ᵉ := ℰ.bwdsRejoin (.once rm) (.once rn)
 
 /-*---------------------
   Semantic equivalence
 ---------------------*-/
 
-/-* Semantic equivalence of contexts *-/
+/-* Semantic equivalence of contexts as a PER *-/
 
 def semCtxt Γ (σ τ : Nat → Val) := ∀ {x A}, Γ ∋ x ∶ A → (σ x, τ x) ∈ ⟦ A ⟧ᵛ
 notation:40 Γ:41 "⊨" σ:41 "~" τ:41 => semCtxt Γ σ τ
@@ -227,39 +227,91 @@ theorem semCtxt.cons {Γ σ τ v w A} (h : (v, w) ∈ ⟦ A ⟧ᵛ) (hστ : Γ 
   | _, _, .here => h
   | _, _, .there mem => hστ mem
 
+theorem semCtxt.sym {Γ σ τ} (h : Γ ⊨ σ ~ τ) : Γ ⊨ τ ~ σ := λ mem ↦ (h mem).sym
+
+theorem semCtxt.trans {Γ ρ σ τ} (hρσ : Γ ⊨ ρ ~ σ) (hστ : Γ ⊨ σ ~ τ) : Γ ⊨ ρ ~ τ :=
+  λ mem ↦ 𝒱.trans (hρσ mem) (hστ mem)
+
 theorem semCtxt.rename {ξ σ τ} {Γ Δ : Ctxt} (hξ : Γ ⊢ ξ ∶ Δ) (h : Γ ⊨ σ ~ τ) : Δ ⊨ σ ∘ ξ ~ τ ∘ ξ :=
   λ mem ↦ h (hξ _ _  mem)
+
+/-* Semantic equivalence of join point contexts as a PER *-/
+
+section
+set_option hygiene false
+local notation:40 Γ:41 "∣" Δ:41 "⊨" js₁:41 "~" js₂:41 => semDtxt Γ Δ js₁ js₂
+inductive semDtxt (Γ : Ctxt) : Dtxt → J → J → Prop where
+  | nil : Γ ∣ ⬝ ⊨ .nil ~ .nil
+  | cons {Δ js₁ js₂ m n A B} : Γ ∣ Δ ⊨ js₁ ~ js₂ →
+    (∀ {σ τ v w}, Γ ⊨ σ ~ τ → (v, w) ∈ ⟦ A ⟧ᵛ → (rejoin (m⦃v +: σ⦄) (substJ σ js₁), rejoin (n⦃w +: τ⦄) (substJ τ js₂)) ∈ ⟦ B ⟧ᵉ) →
+    Γ ∣ Δ ∷ A ↗ B ⊨ .cons m js₁ ~ .cons n js₂
+end
+notation:40 Γ:41 "∣" Δ:41 "⊨" js₁:41 "~" js₂:41 => semDtxt Γ Δ js₁ js₂
+
+theorem semDtxt.sym {Γ Δ js₁ js₂} (h : Γ ∣ Δ ⊨ js₁ ~ js₂) : Γ ∣ Δ ⊨ js₂ ~ js₁ := by
+  induction h
+  case nil => exact .nil
+  case cons h ih => exact .cons ih (λ hστ hvw ↦  .sym (h hστ.sym hvw.sym))
+
+theorem semDtxt.trans {Γ Δ js₁ js₂ js₃} (h₁₂ : Γ ∣ Δ ⊨ js₁ ~ js₂) (h₂₃ : Γ ∣ Δ ⊨ js₂ ~ js₃) : Γ ∣ Δ ⊨ js₁ ~ js₃ := by
+  induction h₁₂ generalizing js₃
+  case nil => exact h₂₃
+  case cons h₁₂ ih =>
+    cases h₂₃; case cons hjs h₂₃ =>
+    refine .cons (ih hjs) (λ hστ hvw ↦  ?_)
+    exact ℰ.trans (h₁₂ hστ hvw) (h₂₃ (semCtxt.trans hστ.sym hστ) (𝒱.trans hvw.sym hvw))
+
+theorem semDtxt.weaken {Γ Δ js₁ js₂ A} (h : Γ ∣ Δ ⊨ js₁ ~ js₂) : Γ ∷ A ∣ Δ ⊨ renameJ succ js₁ ~ renameJ succ js₂ := by
+  induction h <;> constructor; assumption
+  case cons m n _ _ _ ih _ =>
+    intro σ τ v w hστ hvw
+    have e {σ v} {m : Com} : (m⦃(v +: σ) ∘ lift succ⦄) = (m⦃v +: σ ∘ succ⦄) := by
+      apply substComExt _ _ (λ n ↦ ?_); cases n <;> simp [lift]
+    rw [substRenameCom, substRenameCom, substRenameJ, substRenameJ, e, e]
+    exact ih (λ mem ↦ hστ (.there mem)) hvw
 
 /-* Semantic equivalence of values and computations *-/
 
 @[simp] def semVal Γ v w A := ∀ σ τ, Γ ⊨ σ ~ τ → (v⦃σ⦄, w⦃τ⦄) ∈ ⟦ A ⟧ᵛ
-@[simp] def semCom Γ m n B := ∀ σ τ, Γ ⊨ σ ~ τ → (m⦃σ⦄, n⦃τ⦄) ∈ ⟦ B ⟧ᵉ
+@[simp] def semCom Γ Δ m n B := ∀ σ τ, Γ ⊨ σ ~ τ → ∀ js₁ js₂, Γ ∣ Δ ⊨ js₁ ~ js₂ → (rejoin (m⦃σ⦄) (substJ σ js₁), rejoin (n⦃τ⦄) (substJ τ js₂)) ∈ ⟦ B ⟧ᵉ
 notation:40 Γ:41 "⊨" v:41 "~" w:41 "∶" A:41 => semVal Γ v w A
-notation:40 Γ:41 "⊨" m:41 "~" n:41 "∶" B:41 => semCom Γ m n B
+notation:40 Γ:41 "∣" Δ:41 "⊨" m:41 "~" n:41 "∶" B:41 => semCom Γ Δ m n B
 
 /-* Semantic equivalence is a PER *-/
 
-theorem semCtxt.sym {Γ σ τ} (h : Γ ⊨ σ ~ τ) : Γ ⊨ τ ~ σ := λ mem ↦ (h mem).sym
 theorem semVal.sym {Γ v w} {A : ValType} (h : Γ ⊨ v ~ w ∶ A) : Γ ⊨ w ~ v ∶ A :=
   λ _ _ hστ ↦ (h _ _ hστ.sym).sym
-theorem semCom.sym {Γ m n} {B : ComType} (h : Γ ⊨ m ~ n ∶ B) : Γ ⊨ n ~ m ∶ B :=
-  λ _ _ hστ ↦ (h _ _ hστ.sym).sym
+theorem semCom.sym {Γ Δ m n} {B : ComType} (h : Γ ∣ Δ ⊨ m ~ n ∶ B) : Γ ∣ Δ ⊨ n ~ m ∶ B :=
+  λ _ _ hστ _ _ hjs ↦  (h _ _ hστ.sym _ _ hjs.sym).sym
 
-theorem semCtxt.trans {Γ ρ σ τ} (hρσ : Γ ⊨ ρ ~ σ) (hστ : Γ ⊨ σ ~ τ) : Γ ⊨ ρ ~ τ :=
-  λ mem ↦ 𝒱.trans (hρσ mem) (hστ mem)
 theorem semVal.trans {Γ v₁ v₂ v₃} {A : ValType} (h₁₂ : Γ ⊨ v₁ ~ v₂ ∶ A) (h₂₃ : Γ ⊨ v₂ ~ v₃ ∶ A) : Γ ⊨ v₁ ~ v₃ ∶ A :=
   λ _ _ hστ ↦ by refine 𝒱.trans (h₁₂ _ _ hστ) (h₂₃ _ _ (semCtxt.trans hστ.sym hστ))
-theorem semCom.trans {Γ m₁ m₂ m₃} {B : ComType} (h₁₂ : Γ ⊨ m₁ ~ m₂ ∶ B) (h₂₃ : Γ ⊨ m₂ ~ m₃ ∶ B) : Γ ⊨ m₁ ~ m₃ ∶ B :=
-  λ _ _ hστ ↦ by refine ℰ.trans (h₁₂ _ _ hστ) (h₂₃ _ _ (semCtxt.trans hστ.sym hστ))
+theorem semCom.trans {Γ Δ m₁ m₂ m₃} {B : ComType} (h₁₂ : Γ ∣ Δ ⊨ m₁ ~ m₂ ∶ B) (h₂₃ : Γ ∣ Δ ⊨ m₂ ~ m₃ ∶ B) : Γ ∣ Δ ⊨ m₁ ~ m₃ ∶ B :=
+  λ _ _ hστ _ _ hjs ↦ by refine ℰ.trans (h₁₂ _ _ hστ _ _ hjs) (h₂₃ _ _ (semCtxt.trans hστ.sym hστ) _ _ (semDtxt.trans hjs.sym hjs))
 
 /-*---------------------------------------------
   Fundamental theorem of soundness
   of syntactic typing wrt semantic equivalence
 ---------------------------------------------*-/
 
+theorem rejoinJump {Γ Δ js₁ js₂ j A B} (mem : Δ ∋ j ∶ A ↗ B) (h : Γ ∣ Δ ⊨ js₁ ~ js₂) :
+  ∀ {σ τ v w}, Γ ⊨ σ ~ τ → (v, w) ∈ ⟦ A ⟧ᵛ →
+  (rejoin (jump j v) (substJ σ js₁), rejoin (jump j w) (substJ τ js₂)) ∈ ⟦ B ⟧ᵉ := by
+  induction h generalizing j A B
+  case nil => cases mem
+  case cons js₁ js₂ m n _ _ _ h _ =>
+    cases mem
+    case here =>
+      intro σ τ v w hστ hvw; simp
+      refine ℰ.bwd (.rejoin ?_) (.rejoin ?_) (h hστ hvw)
+      all_goals rw [substUnion]; exact .γ
+    case there ih _ mem =>
+      intro σ τ v w hστ hvw; simp
+      refine .bwd (.rejoin .join't) (.rejoin .join't) (ih mem hστ hvw)
+
 theorem soundness {Γ} :
   (∀ (v : Val) A, Γ ⊢ v ∶ A → Γ ⊨ v ~ v ∶ A) ∧
-  (∀ {Δ} (m : Com) B, Γ ∣ Δ ⊢ m ∶ B → Γ ⊨ m ~ m ∶ B) := by
+  (∀ {Δ} (m : Com) B, Γ ∣ Δ ⊢ m ∶ B → Γ ∣ Δ ⊨ m ~ m ∶ B) := by
   refine ⟨λ v A h ↦ ?val, λ m B h ↦ ?com⟩
   mutual_induction h, h
   all_goals intro σ τ hστ
@@ -267,46 +319,56 @@ theorem soundness {Γ} :
   case unit => exact 𝒱.unit
   case inl ih => exact 𝒱.inl (ih σ τ hστ)
   case inr ih => exact 𝒱.inr (ih σ τ hστ)
-  case thunk ih => exact 𝒱.thunk (ih σ τ hστ)
+  case thunk ih => exact 𝒱.thunk (ih σ τ hστ .nil .nil .nil)
+  all_goals intro js₁ js₂ hjs
   case force ih =>
     simp [𝒱] at ih
     let ⟨_, _, h, em, en⟩ := ih σ τ hστ
-    simp [em, en]; exact ℰ.bwd .π .π h
+    simp [em, en]; exact ℰ.bwdRejoin .π .π h
   case lam ih =>
-    refine ℰ.lam (λ v w hA ↦ ?_)
+    refine ℰ.bwdsRejoin .refl .refl (ℰ.lam (λ v w hA ↦ ?_))
     rw [← substUnion, ← substUnion]
-    exact ih (v +: σ) (w +: τ) (semCtxt.cons hA hστ)
+    exact ih (v +: σ) (w +: τ) (semCtxt.cons hA hστ) .nil .nil .nil
   case app ihm ihv =>
-    let ⟨_ ,_, r₁, r₂, hAB⟩ := (ihm σ τ hστ).lam_inv
+    let ⟨_ ,_, r₁, r₂, hAB⟩ := (ihm σ τ hστ .nil .nil .nil).lam_inv
     let hB := hAB _ _ (ihv σ τ hστ)
-    exact ℰ.bwds (.trans' (Evals.app r₁) (.once .β)) (.trans' (Evals.app r₂) (.once .β)) hB
-  case ret ih => exact ℰ.ret (ih σ τ hστ)
+    exact ℰ.bwdsRejoin (.trans' (Evals.app r₁) (.once .β)) (.trans' (Evals.app r₂) (.once .β)) hB
+  case ret ih => exact ℰ.bwdsRejoin .refl .refl (ℰ.ret (ih σ τ hστ))
   case letin ihm ihn =>
-    let ⟨v, w, r₁, r₂, hA⟩ := (ihm σ τ hστ).ret_inv
-    refine ℰ.bwds ?_ ?_ (ihn (v +: σ) (w +: τ) (semCtxt.cons hA hστ))
-    all_goals rw [substUnion]
-    . exact .trans' (Evals.letin r₁) (.once .ζ)
-    . exact .trans' (Evals.letin r₂) (.once .ζ)
+    let ⟨v, w, r₁, r₂, hA⟩ := (ihm σ τ hστ .nil .nil .nil).ret_inv
+    refine ℰ.bwds ?_ ?_ (ihn (v +: σ) (w +: τ) (semCtxt.cons hA hστ) _ _ hjs.weaken)
+    all_goals rw [substUnion, substJDrop]
+    . exact Evals.rejoin (.trans' (Evals.letin r₁) (.once .ζ))
+    . exact Evals.rejoin (.trans' (Evals.letin r₂) (.once .ζ))
   case case ihv ihm ihn =>
     simp [𝒱] at ihv
     match ihv σ τ hστ with
     | .inl ⟨v, w, hA₁, ev, ew⟩ =>
       simp [ev, ew]
-      refine ℰ.bwd ?_ ?_ (ihm (v +: σ) (w +: τ) (semCtxt.cons hA₁ hστ))
-      all_goals rw [substUnion]; exact .ιl
+      refine ℰ.bwd ?_ ?_ (ihm (v +: σ) (w +: τ) (semCtxt.cons hA₁ hστ) _ _ hjs.weaken)
+      all_goals rw [substUnion, substJDrop]; exact .rejoin .ιl
     | .inr ⟨v, w, hA₂, ev, ew⟩ =>
       simp [ev, ew]
-      refine ℰ.bwd ?_ ?_ (ihn (v +: σ) (w +: τ) (semCtxt.cons hA₂ hστ))
-      all_goals rw [substUnion]; exact .ιr
-  case prod ihm ihn => exact ℰ.prod (ihm σ τ hστ) (ihn σ τ hστ)
+      refine ℰ.bwd ?_ ?_ (ihn (v +: σ) (w +: τ) (semCtxt.cons hA₂ hστ) _ _ hjs.weaken)
+      all_goals rw [substUnion, substJDrop]; exact .rejoin .ιr
+  case prod ihm ihn =>
+    exact ℰ.bwdsRejoin .refl .refl (ℰ.prod (ihm σ τ hστ .nil .nil .nil) (ihn σ τ hστ .nil .nil .nil))
   case fst ih =>
-    let ⟨_, _, _, _, r₁, r₂, hB₁⟩ := (ih σ τ hστ).fst
-    exact ℰ.bwds (.trans' (Evals.fst r₁) (.once .π1)) (.trans' (Evals.fst r₂) (.once .π1)) hB₁
+    let ⟨_, _, _, _, r₁, r₂, hB₁⟩ := (ih σ τ hστ .nil .nil .nil).fst
+    exact ℰ.bwdsRejoin (.trans' (Evals.fst r₁) (.once .π1)) (.trans' (Evals.fst r₂) (.once .π1)) hB₁
   case snd ih =>
-    let ⟨_, _, _, _, r₁, r₂, hB₂⟩ := (ih σ τ hστ).snd
-    exact ℰ.bwds (.trans' (Evals.snd r₁) (.once .π2)) (.trans' (Evals.snd r₂) (.once .π2)) hB₂
-  case join ihm ihn => sorry
-  case jump mem _ ihv => sorry
+    let ⟨_, _, _, _, r₁, r₂, hB₂⟩ := (ih σ τ hστ .nil .nil .nil).snd
+    exact ℰ.bwdsRejoin (.trans' (Evals.snd r₁) (.once .π2)) (.trans' (Evals.snd r₂) (.once .π2)) hB₂
+  case join m n _ _ _ _ ihm ihn =>
+    let hn := ihn σ τ hστ (.cons m js₁) (.cons m js₂) (.cons hjs (λ {σ τ v w} hστ hvw ↦ ?hm))
+    case hm =>
+      let hm := ihm (v +: σ) (w +: τ) (semCtxt.cons hvw hστ) _ _ hjs.weaken
+      rw [substRenameJ, substRenameJ,
+          substJExt ((v +: σ) ∘ succ) σ (λ _ ↦ rfl),
+          substJExt ((w +: τ) ∘ succ) τ (λ _ ↦ rfl)] at hm
+      exact hm
+    exact hn
+  case jump mem _ ihv => exact rejoinJump mem hjs hστ (ihv σ τ hστ)
 
 def soundVal {Γ v} {A : ValType} : Γ ⊢ v ∶ A → Γ ⊨ v ~ v ∶ A := soundness.left v A
-def soundCom {Γ Δ m} {B : ComType} : Γ ∣ Δ ⊢ m ∶ B → Γ ⊨ m ~ m ∶ B := soundness.right m B
+def soundCom {Γ Δ m} {B : ComType} : Γ ∣ Δ ⊢ m ∶ B → Γ ∣ Δ ⊨ m ~ m ∶ B := soundness.right m B
