CBPV/RTC.lean
@@ -2,16 +2,18 @@ inductive RTC {A : Type} (R : A → A → Prop) : A → A → Prop
   | refl {a} : RTC R a a
   | trans {a b c} : R a b → RTC R b c → RTC R a c
 
-@[refl] def RTC.rfl {m} := @RTC.refl m
+namespace RTC
 
-def RTC.refl' {A R} (a : A) : RTC R a a := .refl
+@[refl] def rfl {m} := @RTC.refl m
 
-def RTC.trans' {A R} {a b c : A} (rab : RTC R a b) (rbc : RTC R b c) : RTC R a c := by
+def refl' {A R} (a : A) : RTC R a a := .refl
+
+def trans' {A R} {a b c : A} (rab : RTC R a b) (rbc : RTC R b c) : RTC R a c := by
   induction rab
   case refl => exact rbc
   case trans => constructor <;> apply_rules
 
-def RTC.once {A R} {a b : A} (r : R a b) : RTC R a b := .trans r .refl
+def once {A R} {a b : A} (r : R a b) : RTC R a b := .trans r .refl
 
 instance {A} {R : A → A → Prop} : Trans R (RTC R) (RTC R) where
   trans := .trans
@@ -24,3 +26,5 @@ instance {A} {R : A → A → Prop} : Trans R R (RTC R) where
 
 instance {A} {R : A → A → Prop} : Trans (RTC R) R (RTC R) where
   trans r₁ r₂ := .trans' r₁ (.once r₂)
+
+end RTC
